Moved utils file; introduced a variation of trace_always; proved its properties; derived "WF" of states in prod trace from the invariant using it

fairis/trace_utils.v
@@ -1,6 +1,7 @@
 From stdpp Require Import option.
 From Paco Require Import paco1 paco2 pacotac.
 From trillium.fairness Require Export inftraces.
+From trillium.fairness Require Import utils.
 
 Definition trace_implies {S L} (P Q : S → option L → Prop) (tr : trace S L) : Prop :=
   ∀ n, pred_at tr n P → ∃ m, pred_at tr (n+m) Q.
@@ -41,138 +42,161 @@ Proof.
     + by destruct tr; [by destruct Htr as [Htr|Htr]|apply IHn].
 Qed.
 
-Lemma traces_match_flip {S1 S2 L1 L2}
-      (Rℓ: L1 -> L2 -> Prop) (Rs: S1 -> S2 -> Prop)
-      (trans1: S1 -> L1 -> S1 -> Prop)
-      (trans2: S2 -> L2 -> S2 -> Prop)
-      tr1 tr2 :
-  traces_match Rℓ Rs trans1 trans2 tr1 tr2 ↔
-  traces_match (flip Rℓ) (flip Rs) trans2 trans1 tr2 tr1.
-Proof.
-  split.
-  - revert tr1 tr2. cofix CH.
-    intros tr1 tr2 Hmatch. inversion Hmatch; simplify_eq.
-    { by constructor. }
-    constructor; [done..|].
-    by apply CH.
-  - revert tr1 tr2. cofix CH.
-    intros tr1 tr2 Hmatch. inversion Hmatch; simplify_eq.
-    { by constructor. }
-    constructor; [done..|].
-    by apply CH.
-Qed.
 
-Lemma traces_match_impl {S1 S2 L1 L2}
-      (Rℓ1: L1 -> L2 -> Prop) (Rs1: S1 -> S2 -> Prop)
-      (Rℓ2: L1 -> L2 -> Prop) (Rs2: S1 -> S2 -> Prop)
-      (trans1: S1 -> L1 -> S1 -> Prop)
-      (trans2: S2 -> L2 -> S2 -> Prop)
-      tr1 tr2 :
-  (∀ ℓ1 ℓ2, Rℓ1 ℓ1 ℓ2 → Rℓ2 ℓ1 ℓ2) →
-  (∀ s1 s2, Rs1 s1 s2 → Rs2 s1 s2) →
-  traces_match Rℓ1 Rs1 trans1 trans2 tr1 tr2 →
-  traces_match Rℓ2 Rs2 trans1 trans2 tr1 tr2.
-Proof.
-  intros HRℓ HRs. revert tr1 tr2. cofix IH. intros tr1 tr2 Hmatch.
-  inversion Hmatch; simplify_eq.
-  - constructor 1. by apply HRs.
-  - constructor 2; [by apply HRℓ|by apply HRs|done|done|]. by apply IH.
-Qed.
+Definition trace_now {S T} (tr : trace S T) P := pred_at tr 0 P.
+Definition trace_always {S T} (tr : trace S T) P := ∀ n, pred_at tr n P.
+Definition trace_eventually {S T} (tr : trace S T) P := ∃ n, pred_at tr n P.
+Definition trace_until {S T} (tr : trace S T) P Q :=
+  ∃ n, pred_at tr n Q ∧ ∀ m, m < n → pred_at tr m P.
 
-Lemma traces_match_infinite_trace {L1 L2 S1 S2: Type}
-      (Rℓ: L1 -> L2 -> Prop) (Rs: S1 -> S2 -> Prop)
-      (trans1: S1 -> L1 -> S1 -> Prop)
-      (trans2: S2 -> L2 -> S2 -> Prop) tr1 tr2 :
-  traces_match Rℓ Rs trans1 trans2 tr1 tr2 → infinite_trace tr1 → infinite_trace tr2.
-Proof.
-  intros Hmatch Hinf n.
-  specialize (Hinf n) as [tr' Hafter].
-  apply traces_match_flip in Hmatch.
-  by eapply traces_match_after in Hafter as [tr'' [Hafter' _]].
-Qed.
+(* works for possibly finite traces *)
+Definition trace_always' {S T} (tr : trace S T) P := 
+  ∀ n, is_Some (after n tr) -> pred_at tr n P.
 
-Lemma traces_match_traces_implies {S1 S2 L1 L2}
-      (Rℓ: L1 -> L2 -> Prop) (Rs: S1 -> S2 -> Prop)
-      (trans1: S1 -> L1 -> S1 -> Prop)
-      (trans2: S2 -> L2 -> S2 -> Prop)
-      (P1 Q1 : S1 → option L1 → Prop)
-      (P2 Q2 : S2 → option L2 → Prop)
-      tr1 tr2 :
-  traces_match Rℓ Rs trans1 trans2 tr1 tr2 →
-  (∀ s1 s2 oℓ1 oℓ2, Rs s1 s2 →
-                    match oℓ1, oℓ2 with
-                    | Some ℓ1, Some ℓ2 => Rℓ ℓ1 ℓ2
-                    | None, None => True
-                    | _, _ => False
-                    end →
-                    P2 s2 oℓ2 → P1 s1 oℓ1) →
-  (∀ s1 s2 oℓ1 oℓ2, Rs s1 s2 →
-                    match oℓ1, oℓ2 with
-                    | Some ℓ1, Some ℓ2 => Rℓ ℓ1 ℓ2
-                    | None, None => True
-                    | _, _ => False
-                    end → Q1 s1 oℓ1 → Q2 s2 oℓ2) →
-  trace_implies P1 Q1 tr1 → trace_implies P2 Q2 tr2.
-Proof.
-  intros Hmatch HP HQ Htr1.
-  intros n Hpred_at.
-  rewrite /pred_at in Hpred_at.
-  assert (traces_match (flip Rℓ)
-                       (flip Rs)
-                       trans2 trans1
-                       tr2 tr1) as Hmatch'.
-  { by rewrite -traces_match_flip. }
-  destruct (after n tr2) as [tr2'|] eqn:Htr2eq; [|done].
-  eapply (traces_match_after) in Hmatch as (tr1' & Htr1eq & Hmatch); [|done].
-  specialize (Htr1 n).
-  rewrite {1}/pred_at in Htr1.
-  rewrite Htr1eq in Htr1.
-  destruct tr1' as [|s ℓ tr']; inversion Hmatch; simplify_eq; try by done.
-  - assert (P1 s None) as HP1 by by eapply (HP _ _ _ None).
-    destruct (Htr1 HP1) as [m Htr1'].
-    exists m. rewrite pred_at_sum. rewrite pred_at_sum in Htr1'.
-    destruct (after n tr1) as [tr1'|] eqn:Htr1eq'; [|done].
-    eapply (traces_match_after) in Hmatch' as (tr2' & Htr2eq' & Hmatch'); [|done].
-    rewrite Htr2eq'.
-    rewrite /pred_at.
-    rewrite /pred_at in Htr1'.
-    destruct (after m tr1') as [tr1''|] eqn:Htr1eq''; [|done].
-    eapply (traces_match_after) in Hmatch' as (tr2'' & Htr2eq'' & Hmatch''); [|done].
-    rewrite Htr2eq''.
-    destruct tr1''; inversion Hmatch''; simplify_eq; try by done.
-    + by eapply (HQ _ _ None None).
-    + by (eapply (HQ _ _ (Some _) _)).
-  - assert (P1 s (Some ℓ)) as HP1 by by (eapply (HP _ _ _ (Some _))).
-    destruct (Htr1 HP1) as [m Htr1'].
-    exists m. rewrite pred_at_sum. rewrite pred_at_sum in Htr1'.
-    destruct (after n tr1) as [tr1'|] eqn:Htr1eq'; [|done].
-    eapply (traces_match_after) in Hmatch' as (tr2' & Htr2eq' & Hmatch'); [|done].
-    rewrite Htr2eq'.
-    rewrite /pred_at.
-    rewrite /pred_at in Htr1'.
-    destruct (after m tr1') as [tr1''|] eqn:Htr1eq''; [|done].
-    eapply (traces_match_after) in Hmatch' as (tr2'' & Htr2eq'' & Hmatch''); [|done].
-    rewrite Htr2eq''.
-    destruct tr1''; inversion Hmatch''; simplify_eq; try by done.
-    + by eapply (HQ _ _ None None).
-    + by (eapply (HQ _ _ (Some _) _)).
-Qed.
+Lemma trace_always_always' {S T} (tr : trace S T) P:
+  trace_always tr P -> trace_always' tr P.
+Proof. rewrite /trace_always /trace_always'. done. Qed.
 
-Lemma traces_match_after_None {S1 S2 L1 L2}
-      (Rℓ: L1 -> L2 -> Prop) (Rs: S1 -> S2 -> Prop)
-      (trans1: S1 -> L1 -> S1 -> Prop)
-      (trans2: S2 -> L2 -> S2 -> Prop)
-      tr1 tr2 n :
-  traces_match Rℓ Rs trans1 trans2 tr1 tr2 ->
-  after n tr2 = None ->
-  after n tr1 = None.
-Proof.
-  revert tr1 tr2.
-  induction n; intros tr1 tr2; [done|].
-  move=> /= Hm Ha.
-  destruct tr1; first by inversion Hm.
-  inversion Hm; simplify_eq. by eapply IHn.
-Qed.
+Section Match.
+  Context {S1 S2 L1 L2: Type}. 
+
+  Lemma traces_match_impl 
+    (Rℓ1: L1 -> L2 -> Prop) (Rs1: S1 -> S2 -> Prop)
+    (Rℓ2: L1 -> L2 -> Prop) (Rs2: S1 -> S2 -> Prop)
+    (trans1: S1 -> L1 -> S1 -> Prop)
+    (trans2: S2 -> L2 -> S2 -> Prop)
+    tr1 tr2 :
+    (∀ ℓ1 ℓ2, Rℓ1 ℓ1 ℓ2 → Rℓ2 ℓ1 ℓ2) →
+    (∀ s1 s2, Rs1 s1 s2 → Rs2 s1 s2) →
+    traces_match Rℓ1 Rs1 trans1 trans2 tr1 tr2 →
+    traces_match Rℓ2 Rs2 trans1 trans2 tr1 tr2.
+  Proof.
+    intros HRℓ HRs. revert tr1 tr2. cofix IH. intros tr1 tr2 Hmatch.
+    inversion Hmatch; simplify_eq.
+    - constructor 1. by apply HRs.
+    - constructor 2; [by apply HRℓ|by apply HRs|done|done|]. by apply IH.
+  Qed.
+
+  Context (Rℓ: L1 -> L2 -> Prop) (Rs: S1 -> S2 -> Prop)
+      (trans1: S1 -> L1 -> S1 -> Prop) (trans2: S2 -> L2 -> S2 -> Prop). 
+
+  Lemma traces_match_flip tr1 tr2 :
+    traces_match Rℓ Rs trans1 trans2 tr1 tr2 ↔
+      traces_match (flip Rℓ) (flip Rs) trans2 trans1 tr2 tr1.
+  Proof.
+    split.
+    - revert tr1 tr2. cofix CH.
+      intros tr1 tr2 Hmatch. inversion Hmatch; simplify_eq.
+      { by constructor. }
+      constructor; [done..|].
+      by apply CH.
+    - revert tr1 tr2. cofix CH.
+      intros tr1 tr2 Hmatch. inversion Hmatch; simplify_eq.
+      { by constructor. }
+      constructor; [done..|].
+      by apply CH.
+  Qed.
+  
+  Lemma traces_match_infinite_trace tr1 tr2 :
+    traces_match Rℓ Rs trans1 trans2 tr1 tr2 → infinite_trace tr1 → infinite_trace tr2.
+  Proof.
+    intros Hmatch Hinf n.
+    specialize (Hinf n) as [tr' Hafter].
+    apply traces_match_flip in Hmatch.
+    by eapply traces_match_after in Hafter as [tr'' [Hafter' _]].
+  Qed.
+
+  Lemma traces_match_traces_implies 
+    (P1 Q1 : S1 → option L1 → Prop)
+    (P2 Q2 : S2 → option L2 → Prop)
+    tr1 tr2 :
+    traces_match Rℓ Rs trans1 trans2 tr1 tr2 →
+    (∀ s1 s2 oℓ1 oℓ2, Rs s1 s2 →
+                      match oℓ1, oℓ2 with
+                      | Some ℓ1, Some ℓ2 => Rℓ ℓ1 ℓ2
+                      | None, None => True
+                      | _, _ => False
+                      end →
+                      P2 s2 oℓ2 → P1 s1 oℓ1) →
+    (∀ s1 s2 oℓ1 oℓ2, Rs s1 s2 →
+                      match oℓ1, oℓ2 with
+                      | Some ℓ1, Some ℓ2 => Rℓ ℓ1 ℓ2
+                      | None, None => True
+                      | _, _ => False
+                      end → Q1 s1 oℓ1 → Q2 s2 oℓ2) →
+    trace_implies P1 Q1 tr1 → trace_implies P2 Q2 tr2.
+  Proof.
+    intros Hmatch HP HQ Htr1.
+    intros n Hpred_at.
+    rewrite /pred_at in Hpred_at.
+    assert (traces_match (flip Rℓ)
+              (flip Rs)
+              trans2 trans1
+              tr2 tr1) as Hmatch'.
+    { by rewrite -traces_match_flip. }
+    destruct (after n tr2) as [tr2'|] eqn:Htr2eq; [|done].
+    eapply (traces_match_after) in Hmatch as (tr1' & Htr1eq & Hmatch); [|done].
+    specialize (Htr1 n).
+    rewrite {1}/pred_at in Htr1.
+    rewrite Htr1eq in Htr1.
+    destruct tr1' as [|s ℓ tr']; inversion Hmatch; simplify_eq; try by done.
+    - assert (P1 s None) as HP1 by by eapply (HP _ _ _ None).
+      destruct (Htr1 HP1) as [m Htr1'].
+      exists m. rewrite pred_at_sum. rewrite pred_at_sum in Htr1'.
+      destruct (after n tr1) as [tr1'|] eqn:Htr1eq'; [|done].
+      eapply (traces_match_after) in Hmatch' as (tr2' & Htr2eq' & Hmatch'); [|done].
+      rewrite Htr2eq'.
+      rewrite /pred_at.
+      rewrite /pred_at in Htr1'.
+      destruct (after m tr1') as [tr1''|] eqn:Htr1eq''; [|done].
+      eapply (traces_match_after) in Hmatch' as (tr2'' & Htr2eq'' & Hmatch''); [|done].
+      rewrite Htr2eq''.
+      destruct tr1''; inversion Hmatch''; simplify_eq; try by done.
+      + by eapply (HQ _ _ None None).
+      + by (eapply (HQ _ _ (Some _) _)).
+    - assert (P1 s (Some ℓ)) as HP1 by by (eapply (HP _ _ _ (Some _))).
+      destruct (Htr1 HP1) as [m Htr1'].
+      exists m. rewrite pred_at_sum. rewrite pred_at_sum in Htr1'.
+      destruct (after n tr1) as [tr1'|] eqn:Htr1eq'; [|done].
+      eapply (traces_match_after) in Hmatch' as (tr2' & Htr2eq' & Hmatch'); [|done].
+      rewrite Htr2eq'.
+      rewrite /pred_at.
+      rewrite /pred_at in Htr1'.
+      destruct (after m tr1') as [tr1''|] eqn:Htr1eq''; [|done].
+      eapply (traces_match_after) in Hmatch' as (tr2'' & Htr2eq'' & Hmatch''); [|done].
+      rewrite Htr2eq''.
+      destruct tr1''; inversion Hmatch''; simplify_eq; try by done.
+      + by eapply (HQ _ _ None None).
+      + by (eapply (HQ _ _ (Some _) _)).
+  Qed.
+
+  Lemma traces_match_after_None 
+    tr1 tr2 n :
+    traces_match Rℓ Rs trans1 trans2 tr1 tr2 ->
+    after n tr2 = None ->
+    after n tr1 = None.
+  Proof.
+    revert tr1 tr2.
+    induction n; intros tr1 tr2; [done|].
+    move=> /= Hm Ha.
+    destruct tr1; first by inversion Hm.
+    inversion Hm; simplify_eq. by eapply IHn.
+  Qed.
+
+  Lemma traces_match_trace_always'_state_2 tr1 tr2 (P: S2 -> Prop):
+    traces_match Rℓ Rs trans1 trans2 tr1 tr2 ->
+    (forall s1 s2, Rs s1 s2 -> P s2) ->
+    trace_always' tr2 (fun s _ => P s).
+  Proof.
+    intros MATCH IMPL.
+    red. intros n [atr2 AFTER2].
+    red. rewrite AFTER2.
+    eapply traces_match_after in MATCH as (atr1 & AFTER1 & MATCH'); eauto.
+    apply traces_match_first in MATCH'.
+    apply IMPL in MATCH'. by destruct atr2.
+  Qed.     
+
+End Match.
 
 Fixpoint trace_take {S L} (n : nat) (tr : trace S L) : finite_trace S L :=
   match tr with
@@ -268,11 +292,6 @@ Fixpoint finite_trace_to_trace {S L} (tr : finite_trace S L) : trace S L :=
   | tr :tr[ℓ]: s => s -[ℓ]-> (finite_trace_to_trace tr)
   end.
 
-Definition trace_now {S T} (tr : trace S T) P := pred_at tr 0 P.
-Definition trace_always {S T} (tr : trace S T) P := ∀ n, pred_at tr n P.
-Definition trace_eventually {S T} (tr : trace S T) P := ∃ n, pred_at tr n P.
-Definition trace_until {S T} (tr : trace S T) P Q :=
-  ∃ n, pred_at tr n Q ∧ ∀ m, m < n → pred_at tr m P.
 
 Lemma pred_at_after_is_Some {S T} (tr : trace S T) n P :
   pred_at tr n P → is_Some $ after n tr.
@@ -314,34 +333,120 @@ Lemma trace_eventually_cons {S T} s l (tr : trace S T) P :
   trace_eventually tr P → trace_eventually (s -[l]-> tr) P.
 Proof. intros [n HP]. by exists (Datatypes.S n). Qed.
 
-Lemma trace_eventually_stutter_preserves 
-      {St S' L L': Type} (Us: St -> S') (Ul: L -> option L')
-      tr1 tr2 P :
-  upto_stutter Us Ul tr1 tr2 →
-  trace_eventually tr2 P →
-  trace_eventually tr1 (λ s l, P (Us s) (l ≫= Ul)).
-Proof.
-  intros Hstutter [n Heventually].
-  revert tr1 tr2 Hstutter Heventually.
-  induction n as [|n IHn]; intros tr1 tr2 Hstutter Heventually.
-  - punfold Hstutter; [|apply upto_stutter_mono].
-    induction Hstutter.
-    + rewrite /pred_at in Heventually. simpl in *. exists 0. rewrite /pred_at. simpl in *. done.
-    + destruct (IHHstutter Heventually) as [n Heventually'].
-      exists (1 + n). rewrite /pred_at. rewrite after_sum'. simpl.
-      done.
-    + rewrite /pred_at in Heventually. simpl in *. exists 0. rewrite /pred_at. simpl.
-      simplify_eq. rewrite H0. done.
-  - punfold Hstutter; [|apply upto_stutter_mono].
-    induction Hstutter.
-    + rewrite /pred_at in Heventually. simpl in *. exists 0. rewrite /pred_at. simpl in *. done.
-    + destruct (IHHstutter Heventually) as [n' Heventually'].
-      exists (1 + n'). rewrite /pred_at. rewrite after_sum'. simpl.
-      done.
-    + apply trace_eventually_cons.
-      assert (pred_at str n P) as Heventually'.
-      { rewrite /pred_at in Heventually.
-        simpl in *. done. }
-      eapply IHn; [|done].
-      rewrite /upaco2 in H1. destruct H1; [done|done].
+
+Lemma trace_always_inf {S T} (tr : trace S T) P:
+  trace_always tr P -> infinite_trace tr.
+Proof. 
+  intros ALW. red. intros n.
+  destruct (after n tr) eqn:NTH; [done| ].
+  red in ALW. rewrite /pred_at in ALW.
+  specialize (ALW n). by rewrite NTH in ALW.
+Qed. 
+
+
+(* TODO: move, find existing *)
+Lemma forall2_comm {A B: Type} (P: A -> B -> Prop):
+  (forall a b, P a b) <-> (forall b a, P a b).
+Proof. done. Qed.
+
+(* TODO: move, find existing *)
+Lemma ex_all_impl {A: Type} (P: A -> Prop) (Q: Prop):
+  ((exists x, P x) -> Q) <-> (forall x, P x -> Q).
+Proof. set_solver. Qed. 
+
+Lemma trace_always'_state_after {S T} (tr : trace S T) P:
+  trace_always' tr (fun s _ => P s) <-> forall tr' i (AFTER: after i tr = Some tr'), P (trfirst tr').
+Proof. 
+  rewrite /trace_always'.
+  rewrite forall2_comm. apply forall_proper. intros i.
+  rewrite /is_Some. rewrite ex_all_impl. apply forall_proper. intros tr'.
+  apply and_iff_pre. intros AFTER.
+  rewrite /pred_at. rewrite AFTER. by destruct tr'. 
 Qed.
+
+(* TODO: move *)
+Lemma after_after {St L: Type} (tr1 tr2 tr3: trace St L) i j
+  (AFTERi: after i tr1 = Some tr2)
+  (AFTERj: after j tr2 = Some tr3):
+  after (i + j) tr1 = Some tr3.
+Proof. 
+  generalize dependent tr3. induction j.
+  { simpl. rewrite Nat.add_0_r. congruence. }
+  intros. 
+  rewrite -Nat.add_1_r in AFTERj. rewrite after_sum' in AFTERj.
+  destruct (after j tr2) eqn:Aj; [| done].
+  specialize (IHj _ eq_refl).
+  rewrite Nat.add_succ_r -Nat.add_1_r. by rewrite after_sum' IHj.
+Qed. 
+
+Lemma trace_always'_after {S T} (tr tr' : trace S T) i P
+  (AFTER: after i tr = Some tr'):
+  trace_always' tr P -> trace_always' tr' P.
+Proof. 
+  rewrite /trace_always'. intros ALW n [atr' AFTER'].
+  opose proof * (after_after tr tr') as AFTER''; eauto.
+  ospecialize * ALW.
+  { red. eexists. apply AFTER''. }
+  red in ALW. rewrite AFTER'' in ALW.
+  red. rewrite AFTER'. done.
+Qed. 
+
+Section Upto.
+  Context {St S' L L': Type} (Us: St -> S') (Ul: L -> option L'). 
+
+  Lemma trace_eventually_stutter_preserves           
+    tr1 tr2 P :
+    upto_stutter Us Ul tr1 tr2 →
+    trace_eventually tr2 P →
+    trace_eventually tr1 (λ s l, P (Us s) (l ≫= Ul)).
+  Proof.
+    intros Hstutter [n Heventually].
+    revert tr1 tr2 Hstutter Heventually.
+    induction n as [|n IHn]; intros tr1 tr2 Hstutter Heventually.
+    - punfold Hstutter; [|apply upto_stutter_mono].
+      induction Hstutter.
+      + rewrite /pred_at in Heventually. simpl in *. exists 0. rewrite /pred_at. simpl in *. done.
+      + destruct (IHHstutter Heventually) as [n Heventually'].
+        exists (1 + n). rewrite /pred_at. rewrite after_sum'. simpl.
+        done.
+      + rewrite /pred_at in Heventually. simpl in *. exists 0. rewrite /pred_at. simpl.
+        simplify_eq. rewrite H0. done.
+    - punfold Hstutter; [|apply upto_stutter_mono].
+      induction Hstutter.
+      + rewrite /pred_at in Heventually. simpl in *. exists 0. rewrite /pred_at. simpl in *. done.
+      + destruct (IHHstutter Heventually) as [n' Heventually'].
+        exists (1 + n'). rewrite /pred_at. rewrite after_sum'. simpl.
+        done.
+      + apply trace_eventually_cons.
+        assert (pred_at str n P) as Heventually'.
+        { rewrite /pred_at in Heventually.
+          simpl in *. done. }
+        eapply IHn; [|done].
+        rewrite /upaco2 in H1. destruct H1; [done|done].
+  Qed.
+
+  (* TODO: move? *)
+  Lemma upto_stutter_trfirst btr str
+    (CORR: upto_stutter Us Ul btr str):
+    trfirst str = Us (trfirst btr). 
+  Proof.
+    punfold CORR; [| apply upto_stutter_mono]. by inversion CORR.
+  Qed. 
+
+  Lemma upto_preserves_trace_always'_state
+    tr1 tr2 (P: S' -> Prop) :
+    upto_stutter Us Ul tr1 tr2 →
+    trace_always' tr1 (λ s _, P (Us s)) ->
+    trace_always' tr2 (fun s _ => P s).
+  Proof.
+    intros UPTO ALW1.
+    red. intros n2 [atr2 AFTER2]. red. rewrite AFTER2.
+    opose proof * upto_stutter_after as (n1 & atr1 & AFTER1 & UPTO'); eauto.
+    enough (P (trfirst atr2)); [by destruct atr2| ].
+    apply upto_stutter_trfirst in UPTO'. rewrite UPTO'.
+    red in ALW1. ospecialize * ALW1; eauto.
+    red in ALW1. rewrite AFTER1 in ALW1.
+    by destruct atr1. 
+  Qed.
+
+End Upto.
